---
title: "CA3"
author: "ESNCHR001"
format: "pdf"
---

# Question 1:

Let $X~N_p(\mu,\Sigma)$ with $|\Sigma|>0$. Using the spectral decomposition of the covariance matrix, prove that

$$
(X-\mu)'\Sigma^{-1}(X-\mu)\ ~\ \chi_p^2
$$

1.  Start with $Σe_i=λ_ie_i$ and note that Σ is positive definite.

$$
\Sigma e_p = \lambda_pe_p \newline 
[\Sigma e_1 ....\Sigma e_p] \newline 
[\lambda_i e_1 ....\lambda_p e_p] \newline 
[\lambda_i e_1 ....\lambda_p e_p] = e_p D_p \newline
$$

$$
\Sigma e_p = e_p D_p \newline
\Sigma^{-1} = e_p\ D_p^{-1}\ e_p^{-1}\ \newline
\Sigma^{-1} = e_p\ D_p^{-1}\ e_p' \newline
\Sigma^{-1} = \sum_{i=1}^{p}\ e_i\ \lambda_i^{-1}\ e_i' \ \ (1)
$$

$$ 
\Sigma = e_p\ D_p\ e_p^{-1} \newline
\Sigma = e_p\ D_p\ e_p' \newline 
\Sigma = e_p\ D_p\ e_p^{-1} \newline
\Sigma = \sum_{i=1}^{p}\ e_i\ \lambda_i\ e_i'\ \ \ (2)
$$

2.  Using this, rewrite $(X-\mu)' \Sigma^{-1}\ (X-\mu)$ as the sum of p squared variables

$$
(X-\mu)' \Sigma^{-1}\ (X-\mu) \newline
= (X-\mu)'\ (\sum_{i=1}^{p}\ e_i\ \lambda_i^{-1}\ e_i')\ (X-\mu) \ \ (1)\newline
= \sum_{i=1}^{p} \lambda_i^{-1}\ (X-\mu)'\ e_i\ e_i'\ (X-\mu) \newline
= \sum_{i=1}^{p} \lambda_i^{-1}\ [e_i'\ (X-\mu)]^2 \newline
= \sum_{i=1}^{p} [\frac{1}{\sqrt{\lambda_i}}\ e_i'\ (X-\mu)]^2 \newline
$$

3.  Showing that this vector i.e. $[\frac{1}{\sqrt{\lambda_i}}\ e_i'\ (X-\mu)]$ is a multivariate normal with zero mean and identity covariance

$$
A\ X \sim N_q (A\mu,\ A\Sigma A') \newline
[\frac{1}{\sqrt{\lambda_i}} e_i']\ [X-\mu] \sim N[0, [(\frac{1}{\sqrt{\lambda_i}} e_i')\ \Sigma\ (\frac{1}{\sqrt{\lambda_i}} e_i')']] \newline
$$

Firstly, since X- $\mu$ is centered, we know that the [Mean]{.underline} of this vector is equal to zero.

Secondly, to show that the [Variance]{.underline} of this vector is equal to the identity matrix ...

$$
(\frac{1}{\sqrt{\lambda_i}} e_i')\ \Sigma\ (\frac{1}{\sqrt{\lambda_i}} e_i')' \newline
= \frac{1}{\sqrt{\lambda_i}} e_i'\ \Sigma\ \frac{1}{\sqrt{\lambda_i}} e_i \newline
= \frac{1}{\lambda_i} e_i'\ \Sigma\ e_i ' \newline
= \frac{1}{\sqrt{\lambda_i}} e_i'\ \Sigma\ \frac{1}{\sqrt{\lambda_i}} e_i \newline
= \frac{1}{\sqrt{\lambda_i}} e_i'\ (\sum_{i=1}^{p}\ e_i\ \lambda_i\ e_i')\ \frac{1}{\sqrt{\lambda_i}} e_i \ \ \ (2)\newline
= \frac{1}{\lambda_i}\ \sum_{i=1}^{p}\ e_i'\  e_i\ \lambda_i\ e_i'\ e_i \newline
= \sum_{i=1}^{p}\ \frac{1}{\lambda_i}\ I \  \lambda_i\ I \newline
= \frac{1}{\lambda_i}\ \sum_{i=1}^{p}\ I \  \lambda_i\ I
$$
